Add definitions/compset for parsing + inference together

typing/pure_inference_testScript.sml
@@ -5,13 +5,58 @@ val _ = new_theory "pure_inference_test";
 
 (********************)
 
+Definition parse_and_infer_def:
+  parse_and_infer parse ns str =
+    let parsed = parse str in do
+      (ty, as, cs) <- infer ns LN parsed;
+      if ¬ null as then fail else return ();
+      subs <- solve cs;
+      sub_ty <<- subst_solution subs ty;
+      (vars, _, gen_ty) <<- generalise 0 0 LN FEMPTY sub_ty;
+      res_ty <- oreturn $ type_of gen_ty;
+      return (vars, res_ty)
+    od 0
+End
+
+Definition option_datatype_def[simp]:
+  option_datatype : typedef = (1n, [("Nothing", []); ("Just", [TypeVar 0])])
+End
+
+Definition nat_datatype_def[simp]:
+  nat_datatype nat_id : typedef = (0n, [("Z", []) ;("S", [TypeCons nat_id []])])
+End
+
+Definition list_datatype_def[simp]:
+  list_datatype list_id : typedef =
+    (1n, [("Nil", []); ("Cons", [TypeVar 0; TypeCons list_id [TypeVar 0]])])
+End
+
+Definition simple_ns_def[simp]:
+  simple_ns = (
+    [] : exndef , (* no exceptions *)
+    [option_datatype; nat_datatype 1; list_datatype 2] (* options, nats, lists *)
+  )
+End
+
+(********************)
+
+Definition example_2_def[simp]:
+  example_2 = "(lam (m) (let y m (let x (app y (cons True)) x)))"
+End
+
 Definition example_2_exp_def[simp]:
+  example_2_exp = parse_cexp example_2
+End
+
+Theorem example_2_exp:
   example_2_exp =
     pure_cexp$Lam () ["m"] $
       Let () "y" (Var () "m") $
         Let () "x" (App () (Var () "y") [Prim () (Cons "True") []]) $
          Var () "x"
-End
+Proof
+  simp[] >> CONV_TAC pure_parse_infer_eval
+QED
 
 Definition example_2_infer_def[simp]:
   example_2_infer = infer ([], [(0, [ ("True", []) ; ("False", []) ])])
@@ -29,7 +74,7 @@ Theorem example_2_infer:
         Unify () (CVar 2) (Function (PrimTy Bool) (CVar 3))
       ]), 5)
 Proof
-  simp[] >> CONV_TAC pure_infer_eval
+  simp[] >> CONV_TAC pure_parse_infer_eval
 QED
 
 Definition example_2_solve_def[simp]:
@@ -50,7 +95,7 @@ Theorem example_2_solve:
       5)
   )
 Proof
-  simp[] >> CONV_TAC pure_infer_eval
+  simp[] >> CONV_TAC pure_parse_infer_eval
 QED
 
 Definition example_2_solved_def[simp]:
@@ -63,7 +108,14 @@ End
 Theorem example_2_solved:
   example_2_solved = Function (Function (PrimTy Bool) (CVar 3)) (CVar 3)
 Proof
-  simp[] >> CONV_TAC pure_infer_eval
+  simp[] >> CONV_TAC pure_parse_infer_eval
+QED
+
+Theorem example_2_overall:
+  parse_and_infer parse_cexp simple_ns example_2 =
+  return (1, Function (Function (PrimTy Bool) (TypeVar 0)) (TypeVar 0)) 5
+Proof
+  simp[parse_and_infer_def] >> CONV_TAC pure_parse_infer_eval
 QED
 
 (********************)
